\input{Soal/18 random 8 inequality}
\begin{solusi}
    Since the expression is symmetric, then we can assume WLOG $a \ge b \ge c$. Hence
    \begin{align*}
        a^2 \ge b^2 \ge c^2  \text{ and }
        \dfrac{1}{a^2+b^2+2c^2} \ge \dfrac{1}{a^2+2b^2+c^2} \ge \dfrac{1}{2a^2+b^2+c^2}.
    \end{align*}
    Hence by Rearrangement Inequality
    \begin{align*}
        \cycsum \dfrac{a^2}{a^2+b^2+2c^2} \ge  \cycsum \dfrac{c^2}{a^2+b^2+2c^2} \text{ and }
        \cycsum \dfrac{b^2}{a^2+b^2+2c^2} \ge  \cycsum \dfrac{c^2}{a^2+b^2+2c^2}
    \end{align*}
    thus adding those expressions
    \begin{align*}
        \cycsum \dfrac{a^2+b^2}{a^2+b^2+2c^2} &\ge \cycsum \dfrac{2c^2}{a^2+b^2+2c^2} & (Rearrangement)
    \end{align*}   
    hence we have
    \begin{align*}
        \cycsum\left( \dfrac{(a+b)^2}{c^2+ab} - 2\right)
        &= \cycsum \dfrac{a^2+2ab+b^2-2c^2-2ab}{c^2+ab}\\
        &\ge \cycsum \dfrac{a^2+b^2-2c^2}{c^2+\frac{1}{2}(a^2+b^2)} & (AM-GM)\\
        &= 2\cycsum \left(\dfrac{a^2+b^2}{a^2+b^2+2c^2} - \dfrac{2c^2}{a^2+b^2+2c^2}\right)\\
        &\ge 0 & (Rearrangement) \\
        \implies \cycsum\dfrac{(a+b)^2}{c^2+ab} &\ge \cycsum 2 = 6
    \end{align*}
    where the equality happens when $a=b=c$. QED.
\end{solusi}